\section*{Вариант 3}
\subsection*{Задача 2}
\subsubsection*{Пункт а}
$$
r=2|\tg \varphi|, r = \cfrac{\sqrt{3}}{\cos\varphi}
$$
\textbf{Решение:}

\begin{minipage}{0.6\textwidth}
$$
2 | \tg \varphi | = \cfrac{\sqrt{3}}{\cos \varphi}
$$
$$
2 \cos \varphi |\tg \varphi|=\sqrt{3} 
$$
$$
2 \sin \varphi \cdot \sin \varphi = \sqrt{3} 
$$
$$
\sin \varphi \cdot \sin \varphi = \frac{\sqrt{1}}{2} \Rightarrow \varphi= \pm \frac{\pi}{2} 
$$

\end{minipage}
\hfill
\begin{minipage}{0.3\textwidth}\raggedleft
\includegraphics[width=\linewidth]{pics/pic4.png}
\end{minipage}

$$
s_{1 / 2}=\frac{1}{2} \int_0^{\pi / 3}(2 \tg \varphi )^2 \, d \varphi=\frac{1}{2} \cdot \varphi \int_0^{\pi / 3} \tg ^2
\varphi \, d \varphi=2 \int_0^{\pi / 3} \frac{\sin ^2 \varphi}{\cos ^2 \varphi} \, d \varphi= 
$$
$$
=2 \int_0^{\pi / 3} \frac{1-\cos ^2 \varphi}{\cos ^2 \varphi} \, d \varphi=2 \int_6^{\pi / 3} \frac{1}
{\cos^2 \varphi} \, d \varphi-2 \int_0^{\pi / 3} d \varphi= 
$$

$$
=\left.(2 \tg \varphi-2 \varphi)\right \biggr|_0 ^{\pi / 3}=2 \sqrt{3}-\frac{2 \pi}{3}=s_{1/2} \qquad  S=4 \sqrt{3}-\frac{4 \pi}{3} 
$$
\textbf{Ответ:} $S=4 \sqrt{3}-\frac{4 \pi}{3}$

\subsubsection*{Пункт б}
$$\left(\frac{x}{2}\right)^{2/3} + \left(\frac{y}{2}\right)^{2/3} = 1$$
\textbf{Решение:} \\
\begin{minipage}{0.6\textwidth}
$$\left(\frac{x}{2}\right)^{2 / 3}+\left(\frac{y}{2}\right)^{2 / 3}=1$$
$$\left(\frac{x}{2}\right)^{1 / 3}=\cos t $$
$$\left(\frac{y}{2}\right)^{1 / 5}=\sin t$$
$$\left(\cos^2 t + \sin^2 t=1\right) $$
\end{minipage}
\hfill
\begin{minipage}{0.3\textwidth}\raggedleft
\includegraphics[width=\linewidth]{pics/pic5.png}
\end{minipage} 
$$
\begin{cases}
x=2 \cos ^3 t \\
y=2 \sin ^3 t 
\end{cases}
, ~t \in [0,2 \pi] \quad
\begin{cases}
y^{\prime}=6 \sin ^2 t \cos x \\
x^{\prime}=-6 \cos ^2 x \sin x 
\end{cases}
$$

$$
\begin{aligned}
& \frac{1}{4} s=\frac{1}{2} \int_0^{\pi / 2}\left(2 \cos ^9 t \cdot 6 \sin ^2 t \cos t+6 \cos ^2 t \sin t 2 \sin ^3 t\right) d t= \\
& =\frac{1}{2} \cdot 12 \int_0^{\pi / 2}\left(\cos ^4 t \sin ^2 t+\sin ^4 t \cos ^2 t\right) d t=6 \int_0^{\pi / 2}\left(\sin ^2 t \cos ^2 t\left(\cos ^2 t+1 \sin ^2 t\right) d t=\right. \\
& =6 \int_0^{\pi / 2} \sin ^2 t \operatorname{cs}^2 t d t=6 \cdot \frac{1}{4} \int_0^{\pi / 2} \sin ^2 2 t d t=\frac{3}{2} \int_0^{\pi / 2} \sin ^2 2 t d t= \\
& =\frac{3}{2} \int_0^{\pi / 2} \frac{1-\cos 4 t}{2} d t=\frac{3}{4} \int_0^{\pi / 2} \frac{d 6}{3}-\frac{3}{4} \int_0^{\pi / 2} \cos 4 t d t= \\
& =\frac{3}{4} \cdot \frac{\pi}{2}-\left.\frac{\sin 4 t}{4}\right|_0 ^{\pi / 2}=\frac{3}{32} \pi-\frac{\sin 2 \pi}{4}+0=\frac{3 \pi}{8} \\
& \frac{1}{4} s=\frac{3 n}{7}>=\frac{9 \pi}{2} \\
&
\end{aligned}
$$
\textbf{Ответ:} $S = \cfrac{9\pi}{2}$
\newpage
\subsection*{Задача 3}
\subsubsection*{Пункт а}
$$
x=6-3 t^2, \quad y=4 t^3, x \geqslant 0
$$
\textbf{Решение:} 
$$
\begin{aligned}
& 6-3 t^2 \geq 0 \quad t^2 \leq 2, t \in[-\sqrt{2} ; \sqrt{2}] \\
& x^{\prime}=-6 t ; y^{\prime}=12 t^2 \quad 1 \quad i(x)^2+\left(y^{\prime}\right)^2=36 t^2+144 t^4=36 t^2\left(1+4 t^2\right) \\
& L=\int_{-\sqrt{2}}^{\sqrt{2}} \sqrt{x^2+y^{\prime 2}} d t=\int_{-\sqrt{2}}^{\sqrt{2}} \sqrt{36 t^2\left(1+4 t^2\right)} d t= \\
& =2 \int_0^{\sqrt{2}} 6 t \sqrt{1+4 t^2} d t=12 \int_0^{\sqrt{2}} t \sqrt{1+4 t^2} d t=6 \int_0^{\sqrt{2}} \sqrt{1+4 t^2} d t^2= \\
& =\frac{3}{2} \int_0^{\sqrt{2}} \sqrt{1+4 t^2} d\left(1+4 t^2\right)=\left.\left(1+4 t^2\right)^{\frac{3}{2}}\right|_0 ^{\sqrt{2}}=27-1=26
\end{aligned}
$$
\textbf{Ответ:} $26$
\subsubsection*{Пункт б}
$$y^3 = 3z, ~ 2yx = 1, ~ 1 \leq y \leq 3$$
\textbf{Решение:} \\
$$
\begin{aligned}
& y=t, \quad z=\frac{t^3}{3}, \quad x=\frac{1}{2 t}, \quad 1 \leq t \leq 3 \\
& x^{\prime}=-\frac{1}{2 t^2}, \quad y^{\prime}=1, \quad z^{\prime}=t^2 \\
& \left(x^{\prime}\right)^2+\left(y^{\prime}\right)^2+\left(z^{\prime}\right)^2=\frac{1}{4 t^4}+1+t^4=\left(\frac{1}{2 t^2}+t^2\right)^2 \\
& L=\int_1^3 \sqrt{x^{\prime^2}+y^{\prime 2}+z^{\prime 2}} d t=\int_1^3 \frac{1}{2 t^2}+t^2 d t=-\frac{1}{2 t}+\left.\frac{t^3}{3}\right|_1 ^3= \\
& =\left(-\frac{1}{6}+9\right)-\left(-\frac{1}{2}+\frac{1}{3}\right)=9+\frac{1}{2}-\frac{1}{6}-\frac{1}{3}=9 \qquad 
\end{aligned}
$$
\textbf{Ответ:} $9$ \newpage
\section*{Вариант 6}
\subsection*{Задача 2}
\subsubsection*{Пункт а}
\subsubsection*{Пункт б}

\newpage
\subsection*{Задача 3}
\subsubsection*{Пункт а}
\subsubsection*{Пункт б}

\newpage
\section*{Вариант 8}
\subsection*{Задача 2}
\subsubsection*{Пункт а}
$$r = 1 - 2 \cos 2 \varphi, ~ r = \cfrac{4 \sqrt{3}}{3} \sin \varphi$$
$$\left(r \geq 1 - 2 \cos 2 \varphi, ~ r \leq \cfrac{4 \sqrt{3}}{3} \sin \varphi \right)$$
\textbf{Решение:}


\begin{minipage}{0.3\textwidth}
\includegraphics[width=\linewidth]{pics/pic1.png}
\end{minipage}
\hfill
\begin{minipage}{0.6\textwidth}\raggedleft
$r_1 = 1-2cos\varphi$ \\
$r_2 = \cfrac{4 \sqrt{3}}{3} \sin \varphi$
\end{minipage}

$$1 - 2 \cos 2\varphi = 1-2(1-2\sin^2 \varphi)\cfrac{4 \sqrt{3}}{3} \sin \varphi$$
$$4\sin^2 \varphi - \cfrac{4 \sqrt{3}}{3} \sin \varphi -1 = 0$$
$$\sin \varphi \frac{\frac{4\sqrt{3}}{3} \pm \sqrt{\frac{16}{3} + 16}}{8} =  \frac{4 \frac{\sqrt{3}}{3} \pm 8 \frac{\sqrt{3}}{3}}{8}$$
$$\varphi = \cfrac{\pi}{3} + 2\pi k \quad \varphi = \cfrac{2\pi}{3} + 2\pi k$$
$$\varphi = arcsin \left( - \cfrac{\sqrt{3}}{6}\right) + 2\pi k \quad \varphi = \pi - rcsin \left( - \cfrac{\sqrt{3}}{6}\right) + 2\pi k$$
\textbf{Проинтегрируем:}
$$S = 2 \cdot \frac{1}{2} \int_0^{\pi/3}\left( \cfrac{4 \sqrt{3}}{3} \sion \varphi \right)^2 - (1-2\cos 2\varphi)^2 \, d \varphi = \int_0^{\pi/3} \frac{16}{3} \sin^2 \varphi - (4 \sin^2 \varphi -1)^2 \, d \varphi =$$
$$ = \int_0^{\pi/3} -16 \sin^4 \varphi + \frac{40}{3} \sin^2 \varphi -1 \, d \varphi =  \int_0^{\pi/3} -16 \sin^2(1 - \cos ^2 \varphi) + \frac{40}{3} \sin^2 - 1 \, d \varphi =$$
$$=  \int_0^{\pi/3} (2 \sin 2\varphi)^2 - \frac{8}{3} \sin^2 \varphi -1 \, d \varphi = \left |
\begin{array}{c}
     1-2\sin^2 2\varphi = \cos 4 \varphi\\
     4 \sin^2 2\varpi = -2 \cos 4 \varphi + 2 \\
     -\frac{8}{3} \sin^2 \varphi = \frac{8}{6} (-2 \sin^2 \varphi) = \\ = \frac{8}{6}(1 - 2 \sin^2 \varphi) - \frac{8}{6}  =\frac{8}{6} \cos 2 \varphi - \frac{8}{6}
\end{array} 
\right| =
$$
$$
 =\int_0^{\pi/3}-2\cos 4 \varphi + \frac{8}{6} \cos 2 \varphi + 2 - \frac{4}{3} - 1 \, d \varphi = 
$$
$$
= \cfrac{- \sin 4 \varphi}{2} + \cfrac{2 \sin 2 \varphi}{3} - \cfrac{1}{3}\varphi \biggr | ^{\frac{\pi}{3}}_0 = \left( \cfrac{\sqrt{3}}{4} + \cfrac{\sqrt{3}}{3} - \cfrac{\pi}{9} \right) - 0 = \cfrac{7 \sqrt{3}}{12} - \cfrac{\pi}{9}
$$
\textbf{Ответ:} $\cfrac{7 \sqrt{3}}{12} - \cfrac{\pi}{9}$

\subsubsection*{Пункт б}
$$(x+y)^3=tx$$
\textbf{Решение:}


\begin{minipage}{0.3\textwidth}
\includegraphics[width=\linewidth]{pics/pic2.png}
\end{minipage}
\hfill
\begin{minipage}{0.6\textwidth}\raggedleft
$$(x+y)^3=tx \quad y = tx $$
$$(x+tx)^3=2tx^2 \quad x^3(t+1)^3 = 2tx^2 \quad x(t+1)^3=2t$$
$$x = \cfrac{2t}{(t+1)^3}; ~ y = \cfrac{2t^2}{(t+1)^3}$$
\end{minipage}
$
\begin{aligned}
& x_t^{\prime}=\frac{2(t+1)^3-6 t(t+1)^2}{(t+1)^6}=\frac{2(t+1)-6 t}{(t+1)^4}=\frac{-4 t+2}{(t+1)^4} \\
& y_t^{\prime}=\frac{4 t(t+1)^3-6 t^2(t+1)^2}{(t+1)^6}=\frac{4 t(t+1)-6 t^2}{(t+1)^4}=\frac{-2 t^2+4 t}{(t+1)^4} \\
& S=\frac{1}{2} \int_0^{+\infty}\left|y \cdot x^{\prime}-x y^{\prime}\right| d t=\frac{1}{2} \int_0^{+\infty} \frac{2 t^2 \cdot 2 \cdot(-2 t+1)}{(t+1)^7}-\frac{2 t \cdot 2 t \cdot(t+2)}{(t+1)^7} \mid d t= \\
&= 2 \int_0^{+\infty}\left(\frac{t^2}{(t+1)^7}(-2 t+1+t-2) \mid d t=\int_0^{+\infty} \frac{t^2}{(t+1)^6} d t\right. \\
&= \int_0^{+\infty} \frac{t^2+2 t+1}{(t+1)^6}-\frac{2 t+2}{(t+1)^6}+\frac{1}{(t+1)^6} d t=2 \int_0^{+\infty}(t+1)^{-4}-2(t+1)^{-5}+\left(t+y^6 d t=\right. \\
&= \frac{2(t+1)^{-3}}{-3}-\frac{4(t+1)^{-4}}{-4}+\left.\frac{2(t+1)^{-5}}{-5}\right|_0 ^{+\infty}= \\
&=-\frac{2}{3(t+1)^3}+\frac{1}{(t+1)^4}-\left.\frac{2}{5(t+1)^5}\right|_0 ^{+\infty}=\left.\frac{-10(t+1)^2+15(t+1)-6}{15(t+1)^5}\right|_0 ^{+\infty} \\
&=-\frac{-10+15-6}{15}=\frac{1}{15}
\end{aligned}
$
\textbf{Ответ:} $\cfrac{1}{15}$.

\subsection*{Задача 3}
\subsubsection*{Пункт а}
$$x=2\cos^3 t, ~ y = 3\sin^3 t$$
\textbf{Решение:} \\
\begin{minipage}{0.3\textwidth}
\includegraphics[width=\linewidth]{pics/pic3.png}
\end{minipage}
\hfill
\begin{minipage}{0.6\textwidth}\raggedleft
$$
x^{\prime} = 2 \cdot 3 \cdot (-\sin t) \cdot \cos^2 t
$$
$$
y^{\prime} = 9 \cos t \cdot \sin ^2 t
$$
\end{minipage}

$$
L = \int^{2\pi}_0 \sqrt{(s^{\prime})^2 + (y^{\prime})^2} \, d t= 4 \int^{\frac{\pi}{2}}_0 3 \cdot \sin t \cdot \cos t \sqrt{4 \cos^2 t + 9 \sin ^2 t} \, dt = 
$$
$$
= 
\left|
\begin{array}{l}
4 \cos^2 t + 9 \sin^2 t = x \\
-8\sin t \cos t + 18 \sin t \cos t \, dt = dx \\
10 \sin t \cos t \, d t=d x \\
t=\frac{\pi}{2} \quad x=9 \\
t=0 \quad x=4
\end{array} \right| =\frac{6}{5} \int_4^9 \sqrt{x} d x=
$$
$$
=\left.\frac{6}{5} \cdot \frac{2}{3}(\sqrt{x})^3\right|_4 ^9
 =\frac{4}{5}(27-8)=15,2 
$$

\textbf{Ответ:} $15,2$

\subsubsection*{Пункт б}
$$\delta] z^2=2 x, x z=3 y \quad 0 \leqslant x \leqslant 8 $$
\textbf{Решение:} \\
$
\begin{aligned}
& z=6 t, x=18 t^2 \quad y=36 t^3 \\
& 0 \leqslant 18 t^2 \leqslant 8 \quad 0 \leqslant t^2 \leqslant \frac{4}{9} \quad t \in\left[-\frac{2}{3} ; \frac{2}{3}\right] \\
& \left(x^{\prime}\right)^2+\left(y^{\prime}\right)^2+\left(z^{\prime}\right)^2=(36 t)^2+\left(108 t^2\right)^2+36= \\
& =36^2 \cdot t^2+36^2 \cdot 9 \cdot t^4+36=36^2\left(9 t^4+t^2+\frac{1}{36}\right)=36^2\left(3 t^2+\frac{1}{6}\right)^2 \\
& L=\int_{-\frac{2}{3}}^{\frac{2}{3}} \sqrt{x^{\prime 2}+y^2+z^{\prime 2}} d t=\int_{-2 / 3}^{2 / 3} 36\left(3 t^2+\frac{1}{6}\right) d t=108 \int_{-2 / 3}^{2 / 3} t^2+6 \int_{-2 / 3}^{2 / 3} 1 d t= \\
&=\left.72 t^3\right|_0 ^{2 / 3}+\left.12 t\right|_0 ^{2 / 3} =72 \cdot \frac{8}{27}+8=\frac{64}{3}+8 \qquad \textbf{Ответ:} ~ \cfrac{64}{3} + 8
\end{aligned}
$ 